theories/machine_parameters.v
@@ -41,6 +41,7 @@ Class MachineParameters := {
     encodeWordType_correct :
     forall w w', match w,w' with
             | WCap _ _ _ _ _, WCap _ _ _ _ _ => encodeWordType w = encodeWordType w'
+            | WSentry _ _ _ _ _, WSentry _ _ _ _ _ => encodeWordType w = encodeWordType w'
             | WSealRange _ _ _ _ _, WSealRange _ _ _ _ _ => encodeWordType w = encodeWordType w'
             | WSealed _ _, WSealed _ _ => encodeWordType w = encodeWordType w'
             | WInt _, WInt _ => encodeWordType w = encodeWordType w'
@@ -91,6 +92,7 @@ Proof. eapply cancel_inj. Qed.
 
 Section word_type_encoding.
   Definition wt_cap := WCap (O LG LM) Global 0%a 0%a 0%a.
+  Definition wt_sentry := WSentry (O LG LM) Global 0%a 0%a 0%a.
   Definition wt_sealrange := WSealRange (false, false) Global 0%ot 0%ot 0%ot.
   Definition wt_sealed := WSealed 0%ot (SCap (O LG LM) Global 0%a 0%a 0%a).
   Definition wt_int := WInt 0.
@@ -101,7 +103,7 @@ Ltac solve_encodeWordType :=
   | H: _ |- encodeWordType ?x = encodeWordType ?y =>
       try reflexivity
       ; pose proof (encodeWordType_correct x y) as Heq
-      ; unfold wt_cap, wt_int, wt_sealrange, wt_cap; simpl in Heq
+      ; unfold wt_cap, wt_sentry, wt_int, wt_sealrange, wt_cap; simpl in Heq
       ; auto
   end.
 
@@ -109,6 +111,9 @@ Ltac simpl_encodeWordType :=
   match goal with
   | H: _ |- context G [encodeWordType (WCap ?g ?p ?b ?e ?a)] =>
       rewrite (_: encodeWordType (WCap p g b e a) = encodeWordType wt_cap) ; last solve_encodeWordType
+
+  | H: _ |- context G [encodeWordType (WSentry ?g ?p ?b ?e ?a)] =>
+      rewrite (_: encodeWordType (WSentry p g b e a) = encodeWordType wt_cap) ; last solve_encodeWordType
 
   | H: _ |- context G [encodeWordType (WSealRange ?p ?g ?b ?e ?a)] =>
       rewrite (_: encodeWordType (WSealRange p g b e a) = encodeWordType wt_sealrange) ; last solve_encodeWordType
@@ -122,6 +127,11 @@ Ltac simpl_encodeWordType :=
 
 Lemma encodeWordType_correct_cap `{MachineParameters} : forall p g b e a p' g' b' e' a',
   encodeWordType (WCap p g b e a) = encodeWordType (WCap p' g' b' e' a').
+  intros; solve_encodeWordType.
+Qed.
+
+Lemma encodeWordType_correct_sentry `{MachineParameters} : forall p g b e a p' g' b' e' a',
+  encodeWordType (WSentry p g b e a) = encodeWordType (WSentry p' g' b' e' a').
   intros; solve_encodeWordType.
 Qed.
 
